Start adding Itrees family

casestudy/ImpCompCert/Impitrees.v
@@ -1,14 +1,74 @@
 (* Experimenting Imp with itrees-style semantics *)
 (* https://github.com/DeepSpec/InteractionTrees/tree/1569790e28bb5d88381f0763298418d6ccc52eb9/tutorial/Imp.v *)
 
-family Impitrees.Impcommon {
-    family Semantics overrides {
-        (* We want to change the semantics entirely *)
+family Impitrees extends Impzero { }
+
+family Impitrees.Impfrontend {
+    family Semantics *overrides* {
+      (* We want to change the semantics entirely *)
+
+      Context {eff : Type -> Type}.
+      Context {HasImpState : ImpState -< eff}.  
+    
+      Fixpoint denote_expr (e : expr) : itree eff value :=
+        match e with
+        | Var v     => trigger (GetVar v)
+        | Lit n     => ret n
+        | Plus a b  => l <- denote_expr a ;; r <- denote_expr b ;; ret (l + r)
+        | Minus a b => l <- denote_expr a ;; r <- denote_expr b ;; ret (l - r)
+        | Mult a b  => l <- denote_expr a ;; r <- denote_expr b ;; ret (l * r)
+        end.
         
+        Fixpoint denote_imp (s : stmt) : itree eff unit :=
+             match s with
+             | Assign x e =>  v <- denote_expr e ;; trigger (SetVar x v)
+             | Seq a b    =>  denote_imp a ;; denote_imp b
+             | If i t e   =>
+               v <- denote_expr i ;;
+               if is_true v then denote_imp t else denote_imp e
+         
+             | While t b =>
+               while (v <- denote_expr t ;;
+         	           if is_true v
+                      then denote_imp b ;; ret (inl tt)
+                      else ret (inr tt))
+         
+             | Skip => ret tt
+             end.
     }    
 }
 
+(* This prints the things that are broken becuase of the change just made to a family *)
+Print Holes family Impitrees { }. 
+(* 
+Q: In this case, what is broken? 
+1. Simulation proofs 
+2. The "Semantics" nested family in all IR families 
 
-family Impitrees extends Impzero {
-    
-}    
+Q: What is breaks but seems like should be reuseable (i.e not broken)?
+
+Q: How can we display this in an intuitive way? 
+
+Q: How does this list change once we start filling things up 
+   in a family with a higher hierarchy? (e.g in Impfrontend)
+
+*)
+
+family Impitrees.Impshmgen *overrides* { }
+
+family Impitrees.Impshmgen.CorrectnessProofs {
+    Lemma compile_expr_correct : forall {E} e s ts l n,
+      Renv g_imp g_asm ->
+      @eutt E _ _ (sim_rel l n)
+            (Source.interp (denote_expr e) s)
+            (Target.interp (denote_list (compile_expr n e)) ts l).
+    Proof. 
+      ...
+    Qed. 
+
+    Theorem compile_correct {E} {HasExit : Exit -< E} (s : statement) :
+      equivalent (E := E) s (compile s).
+    Proof.
+      ...
+    Qed.
+}
